compiler/backend/proofs/clos_opProofScript.sml
@@ -22,6 +22,210 @@ Proof
   Cases \\ EVAL_TAC
 QED
 
+Theorem dest_Op_thm:
+  dest_Op f x = SOME (i,ys) ⇔
+  ∃tra y. x = Op tra y ys ∧ f y = SOME i
+Proof
+  Cases_on ‘x’ \\ gvs [dest_Op_Nil_def,dest_Op_def,AllCaseEqs()]
+  \\ rw [] \\ eq_tac \\ rw []
+QED
+
+Theorem dest_Op_Nil_thm:
+  dest_Op_Nil f x = SOME i ⇔
+  ∃tra y. x = Op tra y [] ∧ f y = SOME i
+Proof
+  Cases_on ‘x’ \\ gvs [dest_Op_Nil_def,dest_Op_def,AllCaseEqs()]
+  \\ fs [PULL_EXISTS] \\ Cases_on ‘l’ \\ fs []
+QED
+
+Theorem dest_Const_thm:
+  dest_Const x = SOME i ⇔ x = Const i
+Proof
+  Cases_on ‘x’ \\ fs [dest_Const_def]
+QED
+
+Theorem dest_Cons_thm:
+  dest_Cons x = SOME i ⇔ x = Cons i
+Proof
+  Cases_on ‘x’ \\ fs [dest_Cons_def]
+QED
+
+Theorem eq_direct_thm:
+  evaluate ([Op t Equal [x; y]],env,s) = (res,s1) ∧
+  res ≠ Rerr (Rabort Rtype_error) ∧
+  eq_direct x y = SOME z ⇒
+  evaluate ([z],env,s) = (res,s1)
+Proof
+  fs [eq_direct_def]
+  \\ reverse (Cases_on ‘eq_direct_const x y’) \\ fs []
+  THEN1
+   (gvs [eq_direct_const_def,AllCaseEqs(),dest_Op_Nil_thm,dest_Const_thm]
+    \\ fs [evaluate_def,do_app_def]
+    THEN1
+     (Cases_on ‘evaluate ([x],env,s)’ \\ fs [] \\ Cases_on ‘q’ \\ fs []
+      \\ rw [] \\ fs [evaluate_def]
+      \\ imp_res_tac evaluate_SING \\ gvs []
+      \\ cheat)
+    THEN1
+     (Cases_on ‘evaluate ([y],env,s)’ \\ fs [] \\ Cases_on ‘q’ \\ fs []
+      \\ rw [] \\ fs [evaluate_def]
+      \\ imp_res_tac evaluate_SING \\ gvs []
+      \\ cheat)
+    \\ EVAL_TAC \\ rw [] \\ fs [] \\ EVAL_TAC)
+  \\ reverse (Cases_on ‘eq_direct_nil x y’) \\ fs []
+  THEN1
+   (gvs [eq_direct_nil_def,AllCaseEqs(),dest_Op_Nil_thm,dest_Cons_thm]
+    \\ fs [evaluate_def,do_app_def]
+    THEN1
+     (Cases_on ‘evaluate ([x],env,s)’ \\ fs [] \\ Cases_on ‘q’ \\ fs []
+      \\ rw [] \\ fs [evaluate_def]
+      \\ imp_res_tac evaluate_SING \\ gvs [AllCaseEqs()]
+      \\ gvs[do_eq_def,AllCaseEqs(),do_app_def])
+    THEN1
+     (Cases_on ‘evaluate ([y],env,s)’ \\ fs [] \\ Cases_on ‘q’ \\ fs []
+      \\ rw [] \\ fs [evaluate_def]
+      \\ imp_res_tac evaluate_SING \\ gvs [AllCaseEqs()]
+      \\ gvs[do_eq_def,AllCaseEqs(),do_app_def])
+    \\ EVAL_TAC \\ rw [] \\ fs [] \\ EVAL_TAC)
+  \\ fs []
+QED
+
+Theorem dont_lift_Rval:
+  dont_lift x ∧ evaluate ([x],env,s1) = (res,s2) ⇒
+  ∃v. res = Rval [v] ∧ s2 = s1
+Proof
+  cheat
+QED
+
+Theorem evaluate_dont_lift:
+  evaluate ([x],env,s1) = (Rval [v],s2:('a,'b) state) ∧ dont_lift x ⇒
+  evaluate ([x],env1,s) = (Rval [v],s:('a,'b) state)
+Proof
+  cheat
+QED
+
+Theorem lift_exps_acc:
+  ∀xs n binds ys k binds2.
+    lift_exps xs n binds = (ys,k,binds2) ⇒
+    ∃binds1. binds2 = binds ++ binds1
+Proof
+  cheat
+QED
+
+Theorem lift_exps_n:
+  ∀xs n binds ys k binds2.
+    lift_exps xs n binds = (ys,k,binds2) ∧ n = LENGTH binds ⇒
+    k = LENGTH binds2
+Proof
+  cheat
+QED
+
+Theorem lift_exps_thm:
+  ∀xs n binds env s0 ys k vs0 binds2 s1 (s2:('a,'b) state) res0.
+    evaluate (binds,env,s0) = (Rval vs0,s1) ∧
+    evaluate (xs,env,s1) = (res0,s2) ∧ n = LENGTH binds ∧
+    lift_exps xs n binds = (ys,k,binds2) ⇒
+    ∃res.
+      evaluate (binds2,env,s0) = (res,s2) ∧
+      (∀err. res = Rerr err ⇒ res0 = res) ∧
+      ∀ws (s3:('a,'b) state) bind_vals.
+        res = Rval bind_vals ⇒
+        ∃vs. res0 = Rval vs ∧
+             evaluate (ys,bind_vals++ws,s3) = (Rval vs,s3)
+Proof
+  ho_match_mp_tac lift_exps_ind \\ rpt strip_tac
+  THEN1 gvs [lift_exps_def,evaluate_def]
+  \\ gvs [] \\ pop_assum mp_tac
+  \\ simp [lift_exps_def]
+  \\ IF_CASES_TAC
+  THEN1
+   (pairarg_tac \\ gvs [] \\ strip_tac \\ gvs []
+    \\ first_x_assum drule
+    \\ qpat_x_assum ‘evaluate (_::_,_) = _’ mp_tac
+    \\ simp [Once evaluate_CONS]
+    \\ Cases_on ‘evaluate (xs,env,s1)’ \\ gvs []
+    \\ strip_tac \\ gvs [] \\ strip_tac \\ gvs []
+    \\ Cases_on ‘evaluate ([x],env,s1)’ \\ gvs []
+    \\ drule_all dont_lift_Rval
+    \\ strip_tac \\ gvs []
+    \\ Cases_on ‘res’ \\ gvs [] \\ rw []
+    \\ Cases_on ‘q’ \\ gvs []
+    \\ simp [Once evaluate_CONS]
+    \\ drule_all evaluate_dont_lift \\ fs [])
+  \\ Cases_on ‘dest_Op dest_Cons x’ \\ fs []
+  THEN1
+   (pairarg_tac \\ gvs [] \\ strip_tac \\ gvs []
+    \\ qpat_x_assum ‘evaluate _ = _’ mp_tac
+    \\ simp [Once evaluate_CONS]
+    \\ Cases_on ‘evaluate ([x],env,s1)’
+    \\ reverse (Cases_on ‘q’) \\ rw []
+    THEN1
+     (drule lift_exps_acc \\ rw [] \\ fs []
+      \\ full_simp_tac std_ss [GSYM APPEND_ASSOC,APPEND]
+      \\ simp [Once evaluate_APPEND]
+      \\ simp [Once evaluate_CONS])
+    \\ imp_res_tac evaluate_SING \\ gvs []
+    \\ Cases_on ‘evaluate (xs,env,r)’ \\ fs []
+    \\ last_x_assum (qspecl_then [‘env’,‘s0’] mp_tac)
+    \\ simp [Once evaluate_APPEND]
+    \\ rw [] \\ fs []
+    \\ reverse (Cases_on ‘res’) \\ gvs []
+    \\ reverse (Cases_on ‘q’) \\ gvs []
+    \\ drule lift_exps_n \\ rw []
+    \\ imp_res_tac lift_exps_acc \\ gvs []
+    \\ gvs [evaluate_APPEND] \\ gvs [AllCaseEqs()]
+    \\ rw [] \\ pop_assum (qspec_then ‘ws’ strip_assume_tac)
+    \\ gvs [] \\ last_x_assum assume_tac
+    \\ imp_res_tac evaluate_IMP_LENGTH \\ gvs []
+    \\ simp [Once evaluate_CONS]
+    \\ fs [evaluate_def]
+    \\ full_simp_tac std_ss [GSYM APPEND_ASSOC,APPEND] \\ gvs []
+    \\ gvs [EL_APPEND2])
+  \\ rename [‘_ = SOME c’] \\ PairCases_on ‘c’ \\ fs []
+  \\ pairarg_tac \\ fs []
+  \\ pairarg_tac \\ fs []
+  \\ strip_tac \\ gvs [dest_Op_thm,dest_Cons_thm]
+  \\ imp_res_tac lift_exps_acc \\ gvs []
+  \\ first_x_assum drule \\ fs []
+  \\ Cases_on ‘evaluate (c1,env,s1)’ \\ fs [] \\ strip_tac
+  \\ reverse (Cases_on ‘res’) \\ gvs []
+  THEN1
+   (simp [Once evaluate_APPEND]
+    \\ qpat_x_assum ‘evaluate (Op _ _ _ :: _ , _) = _’ mp_tac
+    \\ simp [Once evaluate_CONS]
+    \\ fs [evaluate_def])
+  \\ qpat_x_assum ‘evaluate (Op _ _ _ :: _ , _) = _’ mp_tac
+  \\ simp [Once evaluate_CONS]
+  \\ fs [evaluate_def,do_app_def]
+  \\ reverse (Cases_on ‘q’) THEN1 gvs [] \\ gvs []
+  \\ Cases_on ‘evaluate (xs,env,r)’ \\ fs [] \\ strip_tac
+  \\ imp_res_tac lift_exps_n \\ rw [] \\ gvs []
+  \\ first_x_assum drule_all \\ strip_tac \\ gvs []
+  \\ Cases_on ‘res’ \\ gvs []
+  \\ Cases_on ‘q’ \\ gvs []
+  \\ rw []
+  \\ simp [Once evaluate_CONS]
+  \\ fs [evaluate_def,do_app_def]
+  \\ gvs [evaluate_APPEND] \\ gvs [AllCaseEqs()]
+  \\ gvs [PULL_EXISTS]
+  \\ full_simp_tac std_ss [GSYM APPEND_ASSOC]
+QED
+
+Theorem lift_exps_thm:
+  lift_exps [x] 0 [] = ([y],n,binds) ∧
+  evaluate ([x],env,s1) = (res,s2) ⇒
+  evaluate ([Let None binds y],env,s1) = (res,s2)
+Proof
+  strip_tac
+  \\ drule_at (Pos last) lift_exps_thm
+  \\ fs [evaluate_def]
+  \\ disch_then drule
+  \\ strip_tac \\ fs []
+  \\ reverse (Cases_on ‘res'’) \\ gvs []
+  \\ pop_assum (qspec_then ‘env’ strip_assume_tac)
+  \\ gvs []
+QED
+
 Theorem SmartOp_thm:
   evaluate ([Op t op xs], env, s) = (res,s1) ∧ res ≠ Rerr (Rabort Rtype_error) ⇒
   evaluate ([SmartOp t op xs], env, s) = (res,s1)
@@ -80,15 +284,24 @@ Proof
   \\ reverse (Cases_on ‘dest_Op_Consts x y’) \\ gvs []
   THEN1
    (gvs [AllCaseEqs()]
-    \\ Cases_on ‘x’ \\ fs [dest_Op_Consts_def,dest_Op_def,dest_Const_def]
+    \\ Cases_on ‘x’ \\ fs [dest_Op_Consts_def,dest_Op_Nil_def,dest_Op_def,dest_Const_def]
     \\ Cases_on ‘o'’ \\ fs [dest_Op_Consts_def,dest_Op_def,dest_Const_def]
+    \\ Cases_on ‘l’ \\ fs [dest_Op_Consts_def,dest_Op_def,dest_Const_def]
     \\ Cases_on ‘y’ \\ fs [dest_Op_Consts_def,dest_Op_def,dest_Const_def]
     \\ Cases_on ‘o'’ \\ fs [dest_Op_Consts_def,dest_Op_def,dest_Const_def]
     \\ Cases_on ‘l’ \\ gvs []
-    \\ Cases_on ‘l'’ \\ gvs []
     \\ gvs [int_op_def,AllCaseEqs(),MakeInt_def]
     \\ gvs [evaluate_def,AllCaseEqs(),do_app_def,evaluate_MakeBool]
     \\ gvs [do_eq_def] \\ intLib.COOPER_TAC)
+  \\ last_x_assum mp_tac
+  \\ simp [eq_op_def,GSYM AND_IMP_INTRO]
+  \\ disch_then kall_tac \\ fs [AllCaseEqs()]
+  \\ reverse (Cases_on ‘eq_direct x y’) \\ rw []
+  THEN1 (drule_all eq_direct_thm \\ fs [])
+  \\ gvs [eq_any_def,AllCaseEqs()]
+
+
+
   \\ cheat
 QED
 
